high/Veritas.Verifier.TSLog.fsti
@@ -36,7 +36,7 @@ let g_vlog_of (il: il_vlog): g_vlog =
   I.s_seq il
 
 (* an interleaving is verifiable if the source logs are verifiable *)
-let verifiable (il: il_vlog) = 
+let verifiable (il: il_vlog) =
   VG.verifiable (g_vlog_of il)
 
 (* the clock of an entry in a verifiable idx seq *)
@@ -57,7 +57,7 @@ let its_log = il:il_vlog{verifiable il /\ clock_sorted il}
 
 let hash_verifiable (itsl: its_log) = VG.hash_verifiable (g_vlog_of itsl)
 
-let hash_verifiable_log = 
+let hash_verifiable_log =
   itsl:its_log {hash_verifiable itsl}
 
 val lemma_prefix_verifiable (itsl: its_log) (i:nat{i <= I.length itsl}):
@@ -75,8 +75,8 @@ let clock_sorted_gen (#a:eqtype) (il:I.interleaving a) (c:clock_gen (I.s_seq il)
     forall (i j:I.seq_index il). {:pattern (i2s_map il i); (i2s_map il j)}
       i <= j ==>
         (let i' = i2s_map il i in
-         let j' = i2s_map il j in      
-         c.clock i' `ts_leq` c.clock j') 
+         let j' = i2s_map il j in
+         c.clock i' `ts_leq` c.clock j')
 
 (* create a ts log, generically, given a clock function *)
 val create_gen (#a:eqtype) (vl: sseq a) (c:clock_gen vl)
@@ -87,36 +87,36 @@ val create (gl: VG.verifiable_log): (itsl:its_log{g_vlog_of itsl == gl})
 let state_ops (itsl: il_vlog): seq (state_op) =
   to_state_op_vlog (i_seq itsl)
 
-let key_at (itsl: its_log) (i: I.seq_index itsl): key = 
+let key_at (itsl: its_log) (i: I.seq_index itsl): key =
   V.key_of (I.index itsl i)
-  
+
 let has_next_add_of_key (itsl: its_log) (i: I.seq_index itsl) (k:key): bool =
   has_next (is_add_of_key k) (I.i_seq itsl) i
 
 let next_add_of_key
-  (itsl: its_log) 
-  (i:I.seq_index itsl) 
-  (k:key{has_next_add_of_key itsl i k}): 
-  (j:I.seq_index itsl{j > i && is_add_of_key k (I.index itsl j)}) = 
+  (itsl: its_log)
+  (i:I.seq_index itsl)
+  (k:key{has_next_add_of_key itsl i k}):
+  (j:I.seq_index itsl{j > i && is_add_of_key k (I.index itsl j)}) =
   next_index (is_add_of_key k) (I.i_seq itsl) i
 
-let is_entry_of_key (k:key) (e:vlog_entry): bool = 
+let is_entry_of_key (k:key) (e:vlog_entry): bool =
   key_of e = k
 
-let has_some_entry_of_key (itsl: its_log) (k:key): bool = 
+let has_some_entry_of_key (itsl: its_log) (k:key): bool =
   exists_sat_elems (is_entry_of_key k) (I.i_seq itsl)
 
 let last_idx_of_key (itsl: its_log) (k:key{has_some_entry_of_key itsl k}):
-  I.seq_index itsl = 
+  I.seq_index itsl =
   last_index (is_entry_of_key k) (I.i_seq itsl)
 
 (* does the key k have some add *)
-let has_some_add_of_key (itsl: its_log) (k:key): bool = 
+let has_some_add_of_key (itsl: its_log) (k:key): bool =
   exists_sat_elems (is_add_of_key k) (I.i_seq itsl)
 
 (* the last add index of a key *)
-let last_add_idx (itsl: its_log) (k: key{has_some_add_of_key itsl k}): 
-  (i:I.seq_index itsl{is_add_of_key k (I.index itsl i)}) = 
+let last_add_idx (itsl: its_log) (k: key{has_some_add_of_key itsl k}):
+  (i:I.seq_index itsl{is_add_of_key k (I.index itsl i)}) =
   last_index (is_add_of_key k) (I.i_seq itsl)
 
 (* thread id of the ith entry *)
@@ -135,35 +135,35 @@ val lemma_thread_state_valid (itsl: its_log) (tid: valid_tid itsl)
           [SMTPat (thread_state itsl tid)]
 
 val reveal_thread_state (itsl:il_vlog) (tid: valid_tid itsl)
-  : Lemma (thread_state itsl tid == 
+  : Lemma (thread_state itsl tid ==
            verify (VG.thread_log (s_seq itsl) tid))
 
 (* thread store after processing ts log *)
 let thread_store (itsl: its_log) (tid: valid_tid itsl): vstore =
   Valid?.st (thread_state itsl tid)
 
-let thread_state_pre (itsl: il_vlog) (i: I.seq_index itsl): vtls = 
+let thread_state_pre (itsl: il_vlog) (i: I.seq_index itsl): vtls =
   let tid = thread_id_of itsl i in
   thread_state (I.prefix itsl i) tid
 
-let thread_state_post (itsl: il_vlog) (i: I.seq_index itsl): vtls = 
+let thread_state_post (itsl: il_vlog) (i: I.seq_index itsl): vtls =
   let tid = thread_id_of itsl i in
   thread_state (I.prefix itsl (i + 1)) tid
 
-(* 
- * let tid = thread_id_of itsl i. 
- * this lemma states that state of tid at (i+1) is obtained by the state at (i) 
+(*
+ * let tid = thread_id_of itsl i.
+ * this lemma states that state of tid at (i+1) is obtained by the state at (i)
  * applying the vlog entry at i.
  *)
 val lemma_verifier_thread_state_extend (itsl: il_vlog) (i: I.seq_index itsl):
-  Lemma (thread_state_post itsl i == 
+  Lemma (thread_state_post itsl i ==
          t_verify_step (thread_state_pre itsl i) (I.index itsl i))
 
 
 let mk_vlog_entry_ext (itsl:its_log) (i:I.seq_index itsl)
   : vlog_entry_ext
   =   let ts = thread_state_pre itsl i in
-      let Valid _ st clk _ _ _  = ts in
+      let Valid _ st clk _ _ _ _  = ts in
       let vle = Seq.index (i_seq itsl) i in
       lemma_verifier_thread_state_extend itsl i;
       match vle with
@@ -194,7 +194,7 @@ type neac_log = itsl: its_log {not (is_eac itsl)}
 val eac_boundary (itsl: neac_log):
   (i:I.seq_index itsl{is_eac (I.prefix itsl i) &&
                       not (is_eac (I.prefix itsl (i + 1)))})
-                      
+
 (* if itsl is eac, then any prefix is also eac *)
 val lemma_eac_implies_prefix_eac (itsl: eac_log) (i:nat {i <= I.length itsl}):
   Lemma (requires True)
@@ -204,9 +204,9 @@ val lemma_eac_implies_prefix_eac (itsl: eac_log) (i:nat {i <= I.length itsl}):
 (* if the ts log is eac, then its state ops are read-write consistent *)
 val lemma_eac_implies_state_ops_rw_consistent (itsl: eac_log):
   Lemma (rw_consistent (state_ops itsl))
-  
+
 (* the eac state of a key at the end of an its log *)
-val eac_state_of_key (itsl: its_log) (k:key): eac_state 
+val eac_state_of_key (itsl: its_log) (k:key): eac_state
 
 let eacs_t (itsl:its_log) = k:key -> e:eac_state { e == eac_state_of_key itsl k /\ (is_eac itsl ==> e <> EACFail) }
 let threads_t (itsl:its_log) = t:valid_tid itsl -> v:vtls { Valid? v /\ v == verify (t, Seq.index (I.s_seq itsl) t) }
@@ -269,9 +269,9 @@ let is_eac_state_init (itsl: its_log) (k:key): bool =
   eac_state_of_key itsl k = EACInit
 
 (* is the key k in evicted state in *)
-let is_eac_state_evicted (itsl: its_log) (k:key): bool = 
+let is_eac_state_evicted (itsl: its_log) (k:key): bool =
   EACEvictedMerkle? (eac_state_of_key itsl k) ||
-  EACEvictedBlum? (eac_state_of_key itsl k) 
+  EACEvictedBlum? (eac_state_of_key itsl k)
 
 let eac_state_evicted_value (itsl: its_log) (k:key{is_eac_state_evicted itsl k}): value =
   let st = eac_state_of_key itsl k in
@@ -280,29 +280,29 @@ let eac_state_evicted_value (itsl: its_log) (k:key{is_eac_state_evicted itsl k})
   | EACEvictedBlum v _ _ -> v
 
 (* is the key currently evicted into merkle *)
-let is_eac_state_evicted_merkle (itsl: its_log) (k:key): bool = 
+let is_eac_state_evicted_merkle (itsl: its_log) (k:key): bool =
   let st = eac_state_of_key itsl k in
   match st with
   | EACEvictedMerkle v -> true
   | _ -> false
 
 (* is the key currently evicted into merkle *)
-let is_eac_state_evicted_blum (itsl: its_log) (k:key): bool = 
+let is_eac_state_evicted_blum (itsl: its_log) (k:key): bool =
   let st = eac_state_of_key itsl k in
   match st with
   | EACEvictedBlum v t j -> true
   | _ -> false
 
 (* is the key k in instore state after processing its_log *)
-let is_eac_state_instore (itsl: its_log) (k:key):bool = 
+let is_eac_state_instore (itsl: its_log) (k:key):bool =
   EACInStore? (eac_state_of_key itsl k)
 
-let is_eac_state_active (itsl: its_log) (k:key): bool = 
+let is_eac_state_active (itsl: its_log) (k:key): bool =
   is_eac_state_evicted itsl k ||
   is_eac_state_instore itsl k
 
 (* the extended vlog entry to use for eac checking *)
-val vlog_entry_ext_at (itsl: its_log) (i:I.seq_index itsl): 
+val vlog_entry_ext_at (itsl: its_log) (i:I.seq_index itsl):
   (e:vlog_entry_ext{E.to_vlog_entry e = I.index itsl i})
 
 let eac_state_pre (itsl: its_log) (i:I.seq_index itsl): eac_state =
@@ -315,22 +315,22 @@ let eac_boundary_state_pre (itsl: neac_log): (st:eac_state{EACFail <> st}) =
   lemma_eac_state_of_key_valid (I.prefix itsl i) k;
   eac_state_pre itsl (eac_boundary itsl)
 
-let eac_state_post (itsl: its_log) (i:I.seq_index itsl): eac_state = 
+let eac_state_post (itsl: its_log) (i:I.seq_index itsl): eac_state =
   let k = key_at itsl i in
   eac_state_of_key (I.prefix itsl (i+1)) k
 
-let eac_boundary_entry (itsl: neac_log): vlog_entry = 
+let eac_boundary_entry (itsl: neac_log): vlog_entry =
   I.index itsl (eac_boundary itsl)
 
 (* the eac state transition induced by the i'th entry *)
 val lemma_eac_state_transition (itsl: its_log) (i:I.seq_index itsl):
-  Lemma (eac_state_post itsl i = 
+  Lemma (eac_state_post itsl i =
          eac_add (vlog_entry_ext_at itsl i) (eac_state_pre itsl i))
 
 (* if the ith entry does not involve key k, the eac state of k is unchanged *)
 val lemma_eac_state_same (itsl: its_log) (i: I.seq_index itsl) (k: key):
   Lemma (requires (key_at itsl i <> k))
-        (ensures (eac_state_of_key (I.prefix itsl i) k == 
+        (ensures (eac_state_of_key (I.prefix itsl i) k ==
                   eac_state_of_key (I.prefix itsl (i + 1)) k))
 
 val lemma_eac_boundary_state_transition (itsl: neac_log):
@@ -341,8 +341,8 @@ val lemma_eac_boundary_state_transition (itsl: neac_log):
 
 let lemma_verifier_boundary_thread_state (itsl: neac_log):
   Lemma (requires True)
-        (ensures (thread_state_post itsl (eac_boundary itsl) == 
-                  t_verify_step (thread_state_pre itsl (eac_boundary itsl)) 
+        (ensures (thread_state_post itsl (eac_boundary itsl) ==
+                  t_verify_step (thread_state_pre itsl (eac_boundary itsl))
                                 (I.index itsl (eac_boundary itsl))))
         [SMTPat (eac_boundary itsl)] =
   lemma_verifier_thread_state_extend itsl (eac_boundary itsl)
@@ -357,20 +357,20 @@ val lemma_thread_state_pre_prefix (il:il_vlog) (j:nat{ j <= I.length il}) (i:I.s
 val lemma_thread_state_post_prefix (il:il_vlog) (j:nat{ j <= I.length il}) (i:I.seq_index il { i < j })
   : Lemma (thread_state_post il i == thread_state_post (I.prefix il j) i)
 
-(* If the i'th entry does not go to thread tid, then its state remains unchanged when processing 
+(* If the i'th entry does not go to thread tid, then its state remains unchanged when processing
  * the i'th entry *)
 val lemma_verifier_thread_state_frame (il: il_vlog { I.length il > 0 })
                                       (tid: valid_tid il)
   : Lemma (requires (tid <> thread_id_of il (I.length il - 1)))
           (ensures (thread_state il tid == thread_state (I.hprefix il) tid))
- 
+
 val lemma_verifier_thread_state_extend2 (itsl: il_vlog) (i: I.seq_index itsl) (tid: valid_tid itsl):
   Lemma (requires (tid <> thread_id_of itsl i))
-        (ensures (thread_state (I.prefix itsl (i + 1)) tid == 
+        (ensures (thread_state (I.prefix itsl (i + 1)) tid ==
                   thread_state (I.prefix itsl i) tid))
 
 (* when the eac state of a key is "instore" then there is always a previous add *)
-val lemma_eac_state_active_implies_prev_add (itsl: eac_log) 
+val lemma_eac_state_active_implies_prev_add (itsl: eac_log)
   (k:key{is_eac_state_active itsl k}):
   Lemma (requires True)
         (ensures (has_some_add_of_key itsl k))
@@ -383,27 +383,34 @@ val lemma_eac_state_init_no_entry (itsl: eac_log) (k:key):
 
 (* add method of an eac state *)
 val lemma_eac_state_addm (itsl: eac_log) (k:key{is_eac_state_instore itsl k}):
-  Lemma (E.add_method_of (eac_state_of_key itsl k) = 
+  Lemma (E.add_method_of (eac_state_of_key itsl k) =
          V.addm_of_entry (I.index itsl (last_add_idx itsl k)))
 
 (* the evicted value is always of the correct type for the associated key *)
-val lemma_eac_value_correct_type (itsl: eac_log) (k:key):  
+val lemma_eac_value_correct_type (itsl: eac_log) (k:key):
   Lemma (requires (E.is_eac_state_active (eac_state_of_key itsl k)))
         (ensures is_value_of k (E.value_of (eac_state_of_key itsl k)))
 
 (* value associated with eac state *)
-let eac_state_value (itsl: eac_log) (k:key{is_eac_state_active itsl k}): value_type_of k = 
+let eac_state_value (itsl: eac_log) (k:key{is_eac_state_active itsl k}): value_type_of k =
   let st = eac_state_of_key itsl k in
   lemma_eac_value_correct_type itsl k;
   E.value_of st
 
-(* we never see operations on Root so its eac state is always init *)
+(* we never see operations on Root so its eac state is always init or a special state EACRoot
+ * that we transition to when we see NextEpoch or VerifyEpoch *)
 val lemma_eac_state_of_root_init (itsl: eac_log):
-  Lemma (is_eac_state_init itsl Root)
+  Lemma (ensures (let es = eac_state_of_key itsl Root in
+                  es = EACInit || es = EACRoot))
 
-(* 
- * when the eac state of a key is Init (no operations on the key yet) no 
- * thread contains the key in its store. Valid only for non-root keys 
+(* (Near) inverse of the previous lemma - if the eac state of a key is EACRoot, then that key is Root *)
+val lemma_eac_state_root_implies_root (itsl: eac_log) (k: key):
+  Lemma (requires (eac_state_of_key itsl k = EACRoot))
+        (ensures (k = Root))
+
+(*
+ * when the eac state of a key is Init (no operations on the key yet) no
+ * thread contains the key in its store. Valid only for non-root keys
  * since we start off with the root in the cache of thread 0
  *)
 val lemma_eac_state_init_store (itsl: eac_log) (k: key) (tid:valid_tid itsl):
@@ -411,7 +418,7 @@ val lemma_eac_state_init_store (itsl: eac_log) (k: key) (tid:valid_tid itsl):
         (ensures (not (store_contains (thread_store itsl tid) k)))
 
 (* when the eac state of a key is evicted then no thread contains the key in its store *)
-val lemma_eac_state_evicted_store  (itsl: eac_log) (k: key{is_eac_state_evicted itsl k}) 
+val lemma_eac_state_evicted_store  (itsl: eac_log) (k: key{is_eac_state_evicted itsl k})
   (tid:valid_tid itsl):
   Lemma (not (store_contains (thread_store itsl tid) k))
 
@@ -422,7 +429,7 @@ val lemma_key_in_unique_store2 (itsl: eac_log) (k:key) (tid1 tid2: valid_tid its
                        store_contains (thread_store itsl tid2) k)))
 
 (* when the eac_state of k is instore, then k is in the store of a unique verifier thread *)
-val stored_tid (itsl: eac_log) (k:key{is_eac_state_instore itsl k}): 
+val stored_tid (itsl: eac_log) (k:key{is_eac_state_instore itsl k}):
   (tid: valid_tid itsl{store_contains (thread_store itsl tid) k})
 
 (* uniqueness: k is not in any store other than stored_tid *)
@@ -442,17 +449,17 @@ let stored_add_method (itsl: eac_log) (k:key {is_eac_state_instore itsl k}): add
 val lemma_eac_stored_value (itsl: eac_log) (k: data_key{is_eac_state_instore itsl k}):
   Lemma (eac_state_value itsl k = stored_value itsl k)
 
-(* 
- * for all keys, the add method stored in the store is the same as the add method associated 
+(*
+ * for all keys, the add method stored in the store is the same as the add method associated
  * with eac state
  *)
 val lemma_eac_stored_addm (itsl: eac_log) (k:key{is_eac_state_instore itsl k}):
   Lemma (E.add_method_of (eac_state_of_key itsl k) = stored_add_method itsl k)
-  
+
 (* if k is in a verifier store, then its eac_state is instore *)
 val lemma_instore_implies_eac_state_instore (itsl:eac_log) (k:key{k <> Root}) (tid:valid_tid itsl):
   Lemma (store_contains (thread_store itsl tid) k ==> is_eac_state_instore itsl k)
-         
+
 (* the root is always in thread 0 *)
 val lemma_root_in_store0 (itsl: eac_log{thread_count itsl > 0}):
   Lemma (store_contains (thread_store itsl 0) Root)
@@ -464,7 +471,7 @@ val lemma_root_not_in_store (itsl: eac_log) (tid:valid_tid itsl{tid > 0}):
 val eac_value (itsl: eac_log) (k:key): value_type_of k
 
 (* eac_value is consistent with stored value *)
-val lemma_eac_value_is_stored_value (itsl: eac_log) (k:key) (tid: valid_tid itsl):  
+val lemma_eac_value_is_stored_value (itsl: eac_log) (k:key) (tid: valid_tid itsl):
   Lemma (requires (store_contains (thread_store itsl tid) k))
         (ensures (eac_value itsl k = V.stored_value (thread_store itsl tid) k))
 
@@ -476,16 +483,16 @@ val lemma_ext_evict_val_is_stored_val (itsl: its_log) (i: I.seq_index itsl):
   Lemma (requires (is_evict (I.index itsl i)))
         (ensures (store_contains (thread_store (I.prefix itsl i) (thread_id_of itsl i)) (key_at itsl i) /\
                   is_evict_ext (vlog_entry_ext_at itsl i) /\
-                  V.stored_value (thread_store (I.prefix itsl i) (thread_id_of itsl i)) (key_at itsl i) = 
+                  V.stored_value (thread_store (I.prefix itsl i) (thread_id_of itsl i)) (key_at itsl i) =
                   value_ext (vlog_entry_ext_at itsl i)))
 
-(* if an evict is not the last entry of a key, then there is a add subsequent to the 
+(* if an evict is not the last entry of a key, then there is a add subsequent to the
  * evict *)
-val lemma_evict_has_next_add (itsl: its_log) 
+val lemma_evict_has_next_add (itsl: its_log)
                              (i:I.seq_index itsl)
                              (j:nat { i < j /\ j <= I.length itsl }):
   Lemma (requires (is_evict (I.index itsl i) /\
-                   is_eac (I.prefix itsl j) /\         
+                   is_eac (I.prefix itsl j) /\
                    exists_sat_elems (is_entry_of_key (key_of (I.index itsl i))) (I.i_seq itsl)) /\
                    i < last_idx_of_key itsl (key_of (I.index itsl i)))
         (ensures (has_next_add_of_key itsl i (key_of (I.index itsl i))))
@@ -494,11 +501,15 @@ val lemma_root_never_evicted (itsl: its_log) (i:I.seq_index itsl):
   Lemma (requires (is_evict (I.index itsl i)))
         (ensures (V.key_of (I.index itsl i) <> Root))
 
+val lemma_root_never_added (itsl: its_log) (i: I.seq_index itsl):
+  Lemma (requires (is_add (I.index itsl i)))
+        (ensures (V.key_of (I.index itsl i) <> Root))
+
 (* since the itsl is sorted by clock, the following lemma holds *)
 val lemma_clock_ordering (itsl: its_log) (i1 i2: I.seq_index itsl):
   Lemma (requires (clock itsl i1 `ts_lt` clock itsl i2))
         (ensures (i1 < i2))
-  
+
 (* the state of each key for an empty log is init *)
 val lemma_init_state_empty (itsl: its_log {I.length itsl = 0}) (k: key):
   Lemma (eac_state_of_key itsl k = EACInit)
@@ -514,7 +525,7 @@ val lemma_eac_value_root_init (itsl: eac_log {I.length itsl = 0}) (k:key{k = Roo
 val lemma_addm_ancestor_merkle (itsl: its_log) (i: I.seq_index itsl{is_merkle_add (I.index itsl i)}):
   Lemma (ensures (let AddM _ k' = I.index itsl i in
                   is_merkle_key k'))
-                      
+
 val lemma_evictm_ancestor_merkle (itsl: its_log) (i:I.seq_index itsl{is_evict_to_merkle (I.index itsl i)}):
   Lemma (ensures (let EvictM _ k' = I.index itsl i in
                   is_merkle_key k'))
@@ -523,32 +534,32 @@ val lemma_evictbm_ancestor_merkle (itsl: its_log) (i:I.seq_index itsl{EvictBM? (
   Lemma (ensures (let EvictBM _ k' _ = I.index itsl i in
                   is_merkle_key k'))
 
-val lemma_eac_boundary_inv (itsl: its_log) (i:I.seq_index itsl): 
+val lemma_eac_boundary_inv (itsl: its_log) (i:I.seq_index itsl):
   Lemma (requires (is_eac (I.prefix itsl i) /\
                    not (is_eac (I.prefix itsl (i + 1)))))
-        (ensures (eac_boundary itsl = i)) 
+        (ensures (eac_boundary itsl = i))
 
 ///  If a key is in store, then the last entry of the key cannot be an evict
-/// 
+///
 val lemma_instore_implies_last_entry_non_evict (itsl: eac_log) (k:key) (tid:valid_tid itsl):
   Lemma (requires (store_contains (thread_store itsl tid) k))
-        (ensures (has_some_entry_of_key itsl k ==> 
-                  not (is_evict_to_blum (I.index itsl (last_idx_of_key itsl k))))) 
+        (ensures (has_some_entry_of_key itsl k ==>
+                  not (is_evict_to_blum (I.index itsl (last_idx_of_key itsl k)))))
 
 /// An empty log is eac
-/// 
+///
 val lemma_empty_log_eac (itsl: its_log{I.length itsl = 0})
   : Lemma (ensures (is_eac itsl))
 
-let blum_evict_elem (itsl: its_log) 
-                    (i:I.seq_index itsl{is_evict_to_blum (I.index itsl i)}): ms_hashfn_dom = 
+let blum_evict_elem (itsl: its_log)
+                    (i:I.seq_index itsl{is_evict_to_blum (I.index itsl i)}): ms_hashfn_dom =
   let gl = g_vlog_of itsl in
   let ii = i2s_map itsl i in
   VG.blum_evict_elem gl ii
 
 val lemma_blum_evict_def (itsl: its_log)
                          (i:I.seq_index itsl{is_evict_to_blum (I.index itsl i)}):
-  Lemma (ensures (let tid = thread_id_of itsl i in 
+  Lemma (ensures (let tid = thread_id_of itsl i in
                   let e = I.index itsl i in
                   let k = key_of e in
                   let itsli = I.prefix itsl i in
